examples clean-up

src/examples/bank.v
@@ -1,159 +1,82 @@
-From iris.proofmode Require Import ltac_tactics.
-From iris.bi Require Import monpred.
-From iris.program_logic Require weakestpre.
-From iris.algebra Require Import gmap.
+From iris_named_props Require Import named_props.
+From iris.algebra Require Import excl.
 
-From self.base Require Import primitive_laws.
-From self.lang Require Import lang.
-From self.high Require Import dprop.
+From self.high.lib Require Import abstract_state abstract_state_instances.
+From self.high Require Import protocol wpc_proofmode.
+From self.high Require Import recovery_weakestpre adequacy.
 
-From self.lang Require Export notation lang lemmas tactics syntax.
-From self.algebra Require Import view.
-From self.base Require Import primitive_laws class_instances adequacy.
-From self.high Require Import proofmode wpc_proofmode.
-From self.high Require Import weakestpre_exp weakestpre_at weakestpre_na locations.
-From self.high.modalities Require Import fence.
-From self.high Require Import protocol no_buffer abstract_state_instances.
+From self.examples.lib Require Import gen_maps.
 
-Section FAA_Axiom.
-  Context `{AbstractState ST}.
-  Context `{!nvmG Σ}.
+Definition init: expr :=
+  λ: <>,
+    let: "l" := ref_AT #0 in
+    Flush "l";;
+    FenceSync ;;
+    "l".
 
-  Implicit Types (ℓ : loc) (s : ST) (prot : LocationProtocol ST).
+Definition deposit ℓ: expr :=
+  λ: "n",
+    FAA #ℓ "n" ;;
+    Flush #ℓ ;;
+    FenceSync.
 
-  Definition faa: expr :=
-    rec: "faa" "l" "v_add" :=
-      let: "v_old" := !_AT "l" in
-      if: (CAS "l" "v_old" ("v_old" + "v_add")) then
-        "v_old"
-      else
-        "faa" "l" "v_add".
+(* This [withdraw] is weaker than the in-paper version, but we can
+ * nevertheless verify against the same spec. *)
+Definition withdraw ℓ: expr :=
+  λ: "n",
+    let: "v" := FAA #ℓ (- "n") in
+    (* Flush #ℓ ;; *)
+    (* FenceSync ;; *)
+    "v".
 
-  Lemma wp_faa Q R next ℓ prot `{!ProtocolConditions prot} ss (v_add: Z) st E:
-    {{{
-      ℓ ↦_AT^{prot} (ss) ∗
-      (∀ s_l (v_l: Z) s_p v_p, ∃ P,
-        (  (* The state we write fits in the history. *)
-           (<obj> (prot.(p_full) s_l #v_l -∗ ⌜ s_l ⊑ next s_l ⌝)) ∗
-           (∀ s_n v_n, ⌜ s_l ⊑ s_n ⌝ -∗ prot.(p_full) s_l #v_l -∗
-                       prot.(p_full) s_n v_n ∨
-                         (prot.(p_read) s_n v_n ∧
-                          ∃ s_n' v_n', ⌜ s_n ⊑ s_n' ⌝ ∗ prot.(p_full) s_n' v_n') -∗
-                       ⌜ next s_l ⊑ s_n ⌝) ∗
-           (* Extract the objective knowledge from [p_pers] *)
-           (<obj> (prot.(p_pers) s_p v_p -∗ <obj> P ∗ (P -∗ prot.(p_pers) s_p v_p))) ∗
-           (* Extract from the location we load. *)
-           (<obj> (prot.(p_full) s_l #v_l ∗ P -∗ prot.(p_read) s_l #v_l ∗ R s_l v_l)) ∗
-           (* Establish the invariant for the value we store. *)
-           (R s_l v_l ==∗ prot.(p_full) (next s_l) #(v_l + v_add) ∗ <obj> P ∗ Q s_l v_l)
-        ))
-    }}}
-      FAA #ℓ #v_add @ st; E
-    {{{ (v_l: Z) s_l, RET #v_l;
-        <fence> Q s_l v_l ∗ ℓ ↦_AT^{prot} (ss ++ [next s_l])
-    }}}.
-    Proof.
-  Admitted.
-End FAA_Axiom.
-
-Section Bank.
-  Context `{!nvmG Σ}.
-
-  Variables (ℓ: loc) (γ: gname).
-
-  (* axiomatized section begins *)
-  Definition trans := (gmap nat nat) → (gmap nat nat).
-  Definition promise := trans → Prop.
-  Variables (nextgen: dProp Σ → dProp Σ) (token: gname → promise → iProp Σ) (rely: gname → promise → iProp Σ).
-
-  Instance rely_persistent prom: Persistent (rely γ prom).
-  Proof. Admitted.
-
-  Hypothesis (token_strengthen: ∀ (prom1 prom2: promise), (∀ tr, prom2 tr → prom1 tr) → token γ prom1 ==∗ token γ prom2).
-  Hypothesis (token_bupd_rely: ∀ (prom: promise), token γ prom ==∗ token γ prom ∗ rely γ prom).
-  Hypothesis (rely_weaken: ∀ (prom1 prom2: promise), (∀ tr, prom1 tr → prom2 tr) → rely γ prom1 -∗ rely γ prom2).
-  (* axiomatized section ends *)
-
-  Definition deposit: expr :=
-    λ: "n",
-      FAA #ℓ "n" ;;
-      Flush #ℓ ;;
-      FenceSync.
-
-  Definition withdraw: expr :=
-    λ: "n",
-      let: "v" := FAA #ℓ (- "n") in
-      (* Flush #ℓ ;; *)
-      (* FenceSync ;; *)
-      "v".
+Section bank_protocol.
+  Context `{!nvmBaseGS Σ Ω, !nvmHighGS Σ Ω, !gen_mapG nat Σ Ω}.
+  Notation state := (list (nat + nat)).
+  Variables (γ: gname).
+  Implicit Types (m m__w: gmap nat nat) (h: state) (v: val).
 
   (* abstract state *)
   Program Instance list_abstract_state T `{!EqDecision T, Countable T} : AbstractState (list T) :=
     { abs_state_relation := prefix }.
 
-  Notation state := (list (nat + nat)).
-
-  (* ghost resource *)
-  Context `{!ghost_mapG Σ nat nat}.
-
   Definition to_auth (h: state): gmap nat nat :=
     omap (λ x, match x with inl n => Some n | _ => None end) $ map_seq 0 h.
 
-  Notation dsum h :=
+  Definition dsum h :=
     (foldl (λ sum x, match x with inl n => sum + n | _ => sum end) 0 h).
-
-  Notation wsum h :=
+  Definition wsum h :=
     (foldl (λ sum x, match x with inr n => sum + n | _ => sum end) 0 h).
 
-  Definition state_match h v: dProp Σ :=
-    ⌜ ∃ (n: nat), #n = v ∧ (wsum h + n)%nat = dsum h ⌝.
+  Definition map_sum m := ([^Nat.add map] _ ↦ n ∈ m, n).
 
-  Definition full_pred h: iProp Σ :=
-    ghost_map_auth γ (DfracOwn 1) (to_auth h) ∗
-    ∃ (m__w: gmap nat nat), ([∗ map] k ↦ n ∈ m__w, ghost_map_elem γ k (DfracOwn 1) n) ∗
-                          ⌜ wsum h = [^(Nat.add) map] n ∈ m__w, n ⌝.
+  (* The sub-map where all keys are less than [l] *)
+  Definition map_take l m := (filter (λ '(k, _), Nat.lt k l) m).
 
-  Definition map_trans k (m: gmap nat nat) :=
-    filter (λ '(k', _), k' ≤ k) m.
+  (* evaluating history leads us to the physical value. *)
+  Definition eval h v:= ∃ (n: nat), #n = v ∧ (wsum h + n)%nat = dsum h .
 
-  Definition map_prom k tr :=
-    ∃ k', k' ≥ k ∧ tr = map_trans k'.
+  (* For every prefix of history, the sum of available tokens is greater than
+   * that of all withdrawals. *)
+  Definition settled (h: state) (m__w: gmap nat nat): Prop :=
+    ∀ i, wsum (take i h) ≤ map_sum (map_take i m__w).
 
-  (* protocol for [ℓ] *)
+  Definition full h: iProp Σ :=
+    "auth" ∷ ghost_map_auth γ (DfracOwn 1) (to_auth h) ∗
+    ∃ (m__w: gmap nat nat),
+      "frags" ∷ ([∗ map] k ↦ n ∈ m__w, ghost_map_elem γ k (DfracOwn 1) n) ∗
+      "%settled" ∷ ⌜ settled h m__w ⌝.
+
   Definition prot : LocationProtocol state :=
-    {| p_full := λ (h : state) v, (state_match h v ∗ ⎡ full_pred h ⎤ )%I;
-      p_read := λ (h : state) v, state_match h v;
-      p_pers := λ (h : state) v, ⎡ token γ (map_prom (length h - 1)) ⎤%I;
+    {| p_full := λ (h : state) v, (⌜ eval h v ⌝ ∗ ⎡ full h ⎤)%I;
+      p_read := λ (h : state) v, ⌜ eval h v ⌝%I;
+      p_pers := λ (h : state) v, ⎡ gmap_token γ (length h) ⎤%I;
       p_bumper h := h |}.
-  Global Instance prot_cond : ProtocolConditions prot.
-  Proof.
-    split; try done; try solve_proper; try apply _.
-    - intros.
-      rewrite /prot /=.
-      rewrite bi.equiv_entails.
-      split.
-      { iIntros "[% ?]". iFrame "∗%". done. }
-      { iIntros "[% H]". iFrame "%".
-        iDestruct ("H" with "[//]") as "[_ $]". }
-    - rewrite /prot /=.
-      iIntros (??) "token".
-      admit.
-    - iIntros.
-      iApply post_crash_flush_pure.
-      done.
-  Admitted.
-
-  Definition is_bank: dProp Σ := ℓ ↦_AT^{prot} [ [] ].
-  Definition receipt (n: nat): dProp Σ := ⎡ ∃ k, ghost_map_elem γ k (DfracOwn 1) n ∗ rely γ (map_prom k) ⎤.
 
   (* auxiliary lemmas *)
-
   Lemma to_auth_lookup_length_None h:
     to_auth h !! length h = None.
   Proof.
-    rewrite /to_auth.
-    rewrite lookup_omap.
-    rewrite bind_None.
+    rewrite lookup_omap bind_None.
     left.
     rewrite lookup_map_seq_None.
     lia.
@@ -170,13 +93,14 @@ Section Bank.
     to_auth h = to_auth (h ++ [inr n]).
   Proof.
     rewrite {2}/to_auth map_seq_snoc omap_insert_None /=; last done.
-    rewrite -omap_delete delete_notin; last (apply lookup_map_seq_None; lia).
+    rewrite -omap_delete delete_id; last (apply lookup_map_seq_None; lia).
     done.
     Qed.
 
   Lemma to_auth_dsum h:
-    dsum h = [^Nat.add map] n ∈ to_auth h, n.
+    dsum h = map_sum (to_auth h).
   Proof.
+    rewrite /dsum /map_sum.
     induction h  as [ | [ n | n ] h IH ] using rev_ind.
     - rewrite /to_auth omap_empty big_opM_empty //.
     - rewrite -to_auth_snoc_insert foldl_snoc.
@@ -186,228 +110,363 @@ Section Bank.
       lia.
   Qed.
 
-  Lemma full_pred_deposit_bupd n h:
-    full_pred h ==∗ full_pred (h ++ [inl n]) ∗ ghost_map_elem γ (length h) (DfracOwn 1) n.
+  Lemma to_auth_lookup h i:
+    to_auth h !! i = (h !! i) ≫= (λ x, match x with inl n => Some n | _ => None end).
   Proof.
-    rewrite /full_pred.
-    iIntros "[auth (% & tokens & %)]".
+    rewrite /to_auth lookup_omap lookup_map_seq_0 //.
+  Qed.
+
+  Lemma map_sum_proper:
+    Proper ((⊆) ==> (≤)) map_sum.
+  Proof.
+    rewrite /Proper => m1 m2 ?.
+    rewrite -(map_difference_union m1 m2) //.
+    rewrite /map_sum big_opM_union; last by apply map_disjoint_difference_r1.
+    lia.
+  Qed.
+
+  Lemma map_take_proper:
+    Proper ((≤) ==> (⊆@{gmap nat nat}) ==> (⊆@{gmap nat nat})) map_take.
+  Proof.
+    rewrite /Proper => i1 i2 ? m1 m2 ?.
+    apply map_subseteq_spec. intros ??.
+    rewrite !map_lookup_filter_Some.
+    intros [? ?].
+    split; last lia.
+    by eapply lookup_weaken.
+  Qed.
+
+  Lemma map_sum_take_le_all m i:
+    map_sum (map_take i m) ≤ map_sum m.
+  Proof. apply map_sum_proper, map_filter_subseteq. Qed.
+
+  Lemma settled_deposit h m__w n:
+    settled h m__w → settled (h ++ [inl n]) m__w.
+  Proof.
+    intros Hsettled i.
+    etrans; last apply Hsettled.
+    destruct (decide (i ≤ length h)).
+    - rewrite take_app_le //.
+    - rewrite take_ge; last (rewrite length_app /=; lia).
+      rewrite /wsum foldl_snoc /=.
+      rewrite take_ge //.
+      lia.
+  Qed.
+
+  Lemma settled_withdraw h m__w n k:
+    m__w !! k = None →
+    k < length h →
+    settled h m__w →
+    settled (h ++ [inr n]) (<[k := n]> m__w).
+  Proof.
+    intros ?? Hsettled i.
+    destruct (decide (i ≤ length h)).
+    - rewrite take_app_le //.
+      etrans; first apply Hsettled.
+      apply map_sum_proper, map_take_proper, insert_subseteq; done.
+    - rewrite take_ge; last (rewrite length_app /=; lia).
+      rewrite /wsum foldl_snoc /=.
+      rewrite /map_take map_filter_insert_True; last lia.
+      rewrite /map_sum big_opM_insert; last by rewrite map_lookup_filter_None; left.
+      rewrite (comm Nat.add).
+      apply Nat.add_le_mono_l.
+      etrans; last apply Hsettled.
+      rewrite take_ge //.
+      lia.
+  Qed.
+
+  Lemma map_take_take_min i j m:
+    map_take i (map_take j m) = map_take (i `min` j) m.
+  Proof. rewrite /map_take map_filter_filter. apply map_filter_ext. intros. lia. Qed.
+
+  Lemma settled_crash h__c h m__w:
+    h__c ⊑ h →
+    settled h m__w →
+    settled h__c (map_take (length h__c) m__w).
+  Proof.
+    intros [h' ->] Hsettled i.
+    rewrite map_take_take_min.
+    etrans; last apply Hsettled.
+    destruct (decide (i ≤ length h__c)).
+    - rewrite Nat.min_l //.
+      rewrite take_app_le //.
+    - rewrite Nat.min_r; last lia.
+      rewrite take_app_le //.
+      rewrite ?take_ge //; try lia.
+  Qed.
+
+  Lemma to_auth_crash h__c h:
+    h__c ⊑ h →
+    map_take (length h__c) (to_auth h) = to_auth h__c.
+  Proof.
+    intros. apply map_eq => i.
+    rewrite map_lookup_filter !to_auth_lookup.
+    destruct (decide (i < length h__c)).
+    - rewrite -?(prefix_lookup_lt h__c h) //.
+      destruct (h__c !! i) as [ [ | ] | ]; rewrite /= ?option_guard_True //.
+    - rewrite (lookup_ge_None_2 h__c i); last lia. simpl.
+      destruct (h !! i) as [ [ | ] | ]; rewrite /= ?option_guard_False //.
+  Qed.
+
+  #[global] Instance prot_cond ℓ : ProtocolConditions ℓ prot.
+  Proof.
+    split; try apply _.
+    - intros h v. rewrite /prot /=.
+      iSplit.
+      + iIntros "[$ $] $".
+      + iIntros "[? impl]". by iApply "impl".
+    - rewrite /prot /=.
+      iIntros "_" (h__p v__p h__f v__f) "% tok [%Heval full]".
+      iDestruct "full" as "[auth (%m__w & frags & %Hsettled)]".
+      iSplit.
+      + iMod (ghost_map_auth_elems_token_nextgen (length h__f)
+               with "auth frags tok") as "NG".
+        { by apply prefix_length. }
+        iModIntro. iApply nextgen_flush_nextgen. iModIntro. iIntros "_".
+        iDestruct "NG" as "(auth & frags & tok)".
+        iFrame.
+        iSplitR; first done.
+        iSplitL "auth".
+        (* TODO: make [ghost_map] lemmas use [map_take] as well. *)
+        { rewrite -{2}(to_auth_crash h__f h__f) //. }
+        iPureIntro.
+        by eapply settled_crash.
+      + iIntros (h__c v__c) "!> % % %".
+        iMod (ghost_map_auth_elems_token_nextgen (length h__c)
+               with "auth frags tok") as "NG".
+        { by apply prefix_length. }
+        iModIntro. iApply nextgen_flush_nextgen. iModIntro. iIntros "_".
+        iDestruct "NG" as "(auth & frags & tok)".
+        iFrame.
+        iSplitR; first done.
+        iSplitL "auth".
+        (* TODO: make [ghost_map] lemmas use [map_take] as well. *)
+        { rewrite -(to_auth_crash h__c h__f) //. }
+        iPureIntro.
+        eapply (settled_crash h__c h__f); done.
+    - rewrite /prot /=. by iIntros (???) "!>".
+  Qed.
+End bank_protocol.
+
+Section bank_spec.
+  Context `{!nvmBaseGS Σ Ω, !nvmHighGS Σ Ω, !PerennialG Σ, !gen_mapG nat Σ Ω}.
+
+  (** Interface assertions. *)
+  Definition is_bank ℓ γ: dProp Σ := ℓ ↦_AT^{prot γ} [ [] ] ∗ persist_lb ℓ (prot γ) [].
+  Definition receipt γ (n: nat): dProp Σ :=
+    ⎡ ∃ k p, ⌜ (k < p)%nat ⌝ ∗ ghost_map_elem γ k (DfracOwn 1) n ∗ gmap_rely γ p ⎤.
+
+  Lemma wp_init:
+    {{{ emp }}}
+      init #()
+  {{{ γ ℓ, RET #ℓ; is_bank ℓ γ }}}.
+  Proof.
+    rewrite /init.
+    iIntros (Φ) "_ HΦ".
+    wp_pures.
+    rewrite wp_wpc. iApply fupd_wpc.
+    iMod (gmap_alloc_empty) as (γ) "[auth tok]".
+    rewrite -wp_wpc.
+    iModIntro.
+    wp_apply (wp_alloc_at #0 [] (prot γ) with "[$auth $tok]").
+    { iSplit; first by iExists 0.
+      iExists ∅.
+      rewrite big_sepM_empty.
+      iPureIntro.
+      split; first done.
+      intros ?.
+      rewrite take_nil /wsum /=.
+      lia. }
+    iIntros (ℓ) "#mapsto".
+    wp_pures.
+    wp_apply (wp_flush_lb ℓ (prot γ) []).
+    { by iApply (mapsto_at_store_lb _ _ []). }
+    iIntros "[_ persistLb]".
+    wp_pures.
+    wp_apply (wp_fence_sync).
+    iModIntro.
+    wp_pures.
+    iModIntro.
+    iApply "HΦ".
+    iFrame "∗#".
+  Qed.
+
+  Variable (ℓ: loc) (γ: gname).
+
+  Lemma receipt_nextgen n:
+    receipt γ n ⊢ <NG> receipt γ n.
+  Proof.
+    rewrite /receipt.
+    iIntros "H".
+    iDestruct "H" as (???) "[elem rely]".
+    iDestruct (gmap_elem_rely_nextgen with "elem rely") as "H"; first done.
+    iModIntro.
+    by iDestruct "H" as "[$ $]".
+  Qed.
+  
+  Lemma deposit_update n h:
+    full γ h ==∗ full γ (h ++ [inl n]) ∗ ghost_map_elem γ (length h) (DfracOwn 1) n.
+  Proof.
+    iIntros "[auth (%m__w & frags & %Hsettled)]".
     iMod (ghost_map_insert (length h) n with "auth") as "[auth $]".
     { apply to_auth_lookup_length_None. }
     rewrite to_auth_snoc_insert.
-    iFrame "auth".
-    iModIntro.
-    iExists m__w.
     iFrame.
-    rewrite foldl_snoc //.
+    iPureIntro.
+    by apply settled_deposit.
   Qed.
 
-  Lemma full_pred_withdraw n (v: nat) h:
-    state_match h #v -∗ ⎡ full_pred h ⎤ -∗ receipt n -∗ ⎡ full_pred (h ++ [inr n]) ⎤ ∗ ⌜ n ≤ v ⌝.
+  Lemma withdraw_impl n (v: nat) h:
+    eval h #v →
+    ⎡ full γ h ⎤ -∗
+    receipt γ n -∗
+    ⎡ full γ (h ++ [inr n]) ⎤ ∗ ⌜ n ≤ v ⌝.
   Proof.
-    rewrite /full_pred -to_auth_snoc_noop.
-    iIntros "%steq [auth (% & tokens & %eq)] (%k & frag & _)".
-    simplify_eq.
+    rewrite /full -to_auth_snoc_noop.
+    iIntros (Heval) "[auth (%m__w & frags & %Hsettled)] (% & % & % & frag & _)".
     rewrite embed_big_sepM.
     iAssert ⌜ m__w !! k = None ⌝%I as "%".
-    { destruct ((m__w !! k)) as [ | ] eqn:?; last done.
-      iPoseProof (big_sepM_lookup _ _ k with "tokens") as "frag'"; first done.
-      iPoseProof (ghost_map_elem_valid_2 with "[$] [$]") as "[% _]".
-      done. }
-    iPoseProof (big_sepM_insert with "[$tokens $frag]") as "tokens"; first done.
+    { destruct (m__w !! k) as [ | ] eqn:Heq; last done.
+      iPoseProof (big_sepM_lookup _ _ k with "frags") as "frag'"; first done.
+      by iPoseProof (ghost_map_elem_valid_2 with "frag frag'") as "[% _]". }
+    iPoseProof (big_sepM_insert with "[$frags $frag]") as "frags"; first done.
     rewrite -embed_big_sepM.
-    iPoseProof (ghost_map_lookup_big with "[$] [$]") as "%".
+    iPoseProof (gen_maps.ghost_map_lookup_big with "auth frags") as "%Hsub".
+    assert (k < length h).
+    { assert (to_auth h !! k = Some n) as Hlook.
+      { eapply lookup_weaken; last done. rewrite lookup_insert decide_True //. }
+      rewrite to_auth_lookup in Hlook.
+      destruct (h !! k) as [ | ] eqn:Heq; simpl in Hlook; last done.
+      apply lookup_lt_Some in Heq. done. }
+    assert (n ≤ v).
+    { destruct Heval as (? & ? & Heval).
+      simplify_eq.
+      rewrite to_auth_dsum in Heval.
+      (* pose proof (to_auth_dsum h) as Hdsum. *)
+      apply map_sum_proper in Hsub.
+      rewrite /map_sum big_opM_insert in Hsub; last done.
+      unfold map_sum in Heval.
+      rewrite -Heval in Hsub.
+      assert (wsum h ≤ map_sum m__w); last (unfold map_sum in *; lia).
+      specialize (Hsettled (length h)).
+      rewrite ?take_ge // in Hsettled.
+      etrans; first apply Hsettled.
+      apply map_sum_take_le_all. }
     iFrame.
-    iSplit.
-    { iExists (<[ k := n ]> m__w).
-      iFrame.
-      iPureIntro.
-      rewrite foldl_snoc /=.
-      rewrite big_opM_insert; last done.
-      lia. }
-    pose proof (to_auth_dsum h) as bigeq.
-    rewrite -(map_difference_union (<[k:=n]> m__w) (to_auth h)) in bigeq; last done.
-    rewrite big_opM_union in bigeq; last by apply map_disjoint_difference_r.
-    iPureIntro.
-    rewrite big_opM_insert in bigeq; last done.
-    destruct steq as (? & ? & ?).
-    simplify_eq.
-    lia.
-  Qed.
-
-  Lemma map_prom_strengthen k1 k2:
-    k1 ≤ k2 → ∀ tr, map_prom k2 tr → map_prom k1 tr.
-  Proof.
-    rewrite /map_prom.
-    intros ??(k' & ? & ?).
-    exists k'.
-    split; last done.
-    lia.
+    iSplit; last done.
+    iPureIntro. by apply settled_withdraw.
   Qed.
 
   Lemma wp_deposit n:
-    {{{ is_bank }}}
-      deposit #n
-    {{{ RET #(); receipt n }}}.
+    {{{ is_bank ℓ γ }}}
+      deposit ℓ #n
+    {{{ RET #(); receipt γ n }}}.
   Proof.
-    rewrite /is_bank.
-    iIntros (?) "#is_bank HΦ".
+    rewrite /is_bank /deposit.
+    iIntros (Φ) "#[mapsto _] HΦ".
     wp_pures.
-    wp_bind (FAA _ _).
-    iApply (wp_faa
-              (λ h _, ⎡ ghost_map_elem γ (length h) (DfracOwn 1) n⎤)%I
-              (λ h v, state_match h #v ∗ ⎡ full_pred h ⎤)%I
-              (λ h, h ++ [inl n]) _ prot).
-    { iSplitL; first iFrame "#".
-      iIntros.
-      iExists (True)%I.
-      iSplitL "".
-      { iIntros "!> _".
-        iPureIntro.
-        by eexists. }
-      iSplitL "".
-      { iIntros (???) "[_ [full1 _]] [[_ [full2 _]] | [_ (% & % & % & [_ [full2 _]])]]";
-          by iPoseProof (ghost_map_auth_valid_2 with "full1 full2") as "[%frac _]". }
-      iSplitL "".
-      { iIntros "!> pers".
-        iSplitL ""; first by iModIntro.
-        iIntros. iFrame. }
-      iSplitL "".
-      { iIntros "!> [full _]".
-        iSplit.
-        - iDestruct "full" as "[? _]".
-          done.
-        - iFrame. }
-      iIntros "[%steq full]".
-      iMod (full_pred_deposit_bupd n with "full") as "[full receipt]".
+    wp_apply (wp_faa
+                (λ σ_l n_l σ_t, ⎡ ghost_map_elem γ (length σ_l) (DfracOwn 1) n ⎤ ∗ ⌜(length σ_l < length σ_t)%nat⌝ ∗ seen_state ℓ σ_l)%I
+                (λ σ_l (n_l: Z), ⌜ eval σ_l #n_l ⌝ ∗ ⎡ full γ σ_l ⎤: dProp Σ)%I
+                [] [] ℓ (prot γ)).
+    { iFrame "mapsto".
+      iIntros (σ_l n_l) "_".
+      iSplitR.
+      { iIntros (??) "!> (% & % & %)". by iExists _. }
+      iExists (σ_l ++ [inl n]).
+      iSplitR.
+      { iIntros "!> _". iPureIntro. by apply prefix_app_r. }
+      iSplitR.
+      { iIntros (σ_n v_n) "_ [_ full] disj".
+        iDestruct "full" as "[auth _]".
+        iDestruct "disj" as "[[_ [auth' _]] | [_ (% & % & % & [_ [auth' _]])]]";
+          iDestruct (ghost_map_auth_valid_2 with "[$] [$]") as %[? _]; done. }
+      iSplitR.
+      { iIntros "!> [%Heval full]". by iFrame. }
+      iIntros "#seen [(%n_l' & % & %) full]".
+      simplify_map_eq.
+      iMod (deposit_update n σ_l with "full") as "[full frag]".
       iModIntro.
-      iFrame.
-      iSplitPure.
-      { rewrite ?foldl_snoc.
-        destruct steq as (?n' & ? & ?).
-        simplify_eq.
-        exists (n' + n).
-        split; first rewrite Nat2Z.inj_add //.
-        lia. }
-      by iModIntro.
-    }
-    iModIntro.
-    iIntros (??) "[frag #mapsto]".
-    iPoseProof (post_fence_flush_free with "frag") as "frag".
+      iFrame "∗#".
+      iPureIntro.
+      rewrite length_app /=.
+      split; last lia.
+      exists (n_l' + n).
+      split.
+      - f_equal. by rewrite Nat2Z.inj_add.
+      - unfold dsum, wsum in *. rewrite !foldl_snoc /=. lia. }
+    iIntros (σ_l σ_t n_l) "[Hfence #mapsto']".
     wp_pures.
-    wp_bind (Flush _).
-    iPoseProof (mapsto_at_store_lb with "mapsto") as "#lb".
-    iApply (weakestpre_exp.wp_flush_lb _ _ _ _ _ ⎡ rely γ (map_prom $ length s_l) ⎤%I with "[$lb]").
-    { iSplit.
-      { iDestruct "is_bank" as (???????) "H".
-        iNamed "H".
-        iAssumption. }
-      iIntros "!>" (???).
-      iExists (True)%I.
-      iSplit; first by iIntros "_ !>!>".
-      iIntros "_".
-      rewrite /p_pers /prot //=.
-      iSplit.
-      - iIntros "[% %eq] pers".
-        iMod (token_strengthen _ (map_prom (length s_l)) with "pers").
-        { apply map_prom_strengthen.
-          assert (length_eq: length s_l + length [@inl nat nat n] = length s_p + length k).
-          { rewrite -?length_app. by f_equiv. }
-          simpl in length_eq.
-          lia. }
-        rewrite length_app //=.
-        replace (_ + 1 - 1) with (length s_l) by lia.
-        iMod (token_bupd_rely with "[$]") as "[? ?]".
-        by iFrame.
-      - iIntros "[% ->] pers".
-        iMod (token_bupd_rely with "[$]") as "[$ rely]".
-        iModIntro.
-        iApply (rely_weaken with "rely").
-        apply map_prom_strengthen.
-        rewrite ?length_app //=.
-        lia.
-    }
-    iIntros "!> post_fence_sync".
-    wp_pures.
-    iApply (weakestpre_exp.wp_fence_sync _ prot with "post_fence_sync").
-    iIntros "!> [_ rely]".
-    iApply "HΦ".
-    iExists (length s_l).
-    iFrame.
+    iDestruct "Hfence" as "(>frag & % & seen)".
+    wp_apply (wp_flush_xchg ℓ (prot γ) with "[$seen frag]"); last first.
+    {  iIntros "receipt".
+       wp_pures.
+       iApply (wp_fence_sync' with "[$]").
+       iNext. iIntros "[_ receipt]". by iApply "HΦ". }
+    iSplitR; first by iNamed "mapsto".
+    iSplitR.
+    { iApply (mapsto_at_store_lb with "mapsto'"). }
+    iIntros (v) "!> $".
+    iIntros (σ_old v_old) "!>".
+    iSplit.
+    - iIntros (?) "tok".
+      rewrite /prot /=.
+      iMod (gmap_token_strengthen (length σ_t) with "tok") as "[$ #rely]".
+      { by apply prefix_length. }
+      iModIntro.
+      iIntros (v_xchg) "!> $".
+      iFrame "∗#".
+      by iPureIntro.
+    - iIntros (?) "token".
+      rewrite /prot /=.
+      iMod (gmap_token_strengthen (length σ_old) with "token") as "[$ #rely]"; first done.
+      iModIntro.
+      iIntros (v_xchg) "!> $".
+      iFrame "∗#".
+      iPureIntro.
+      eapply Nat.lt_le_trans; first done.
+      by apply prefix_length.
   Qed.
 
   Lemma wp_withdraw n:
-    {{{ is_bank ∗ receipt n }}}
-      withdraw #n
-    {{{ (v: Z), RET #v; ⌜ (0 ≤ v)%Z ⌝ }}}.
+    {{{ is_bank ℓ γ ∗ receipt γ n }}}
+      withdraw ℓ #n
+      {{{ (v: Z), RET #v; ⌜ (0 ≤ v)%Z ⌝ }}}.
   Proof.
-    rewrite /is_bank.
-    iIntros (?) "[#is_bank receipt] HΦ".
+    rewrite /withdraw.
+    iIntros (Φ) "[[#mapsto _] receipt] HΦ".
     wp_pures.
-    wp_bind (FAA _ _).
-    iApply (wp_faa
-              (λ h v, state_match h #v)%I
-              (λ h v, state_match h #v ∗ ⎡ full_pred h ⎤)%I
-              (λ h, h ++ [inr n]) _ prot with "[receipt]").
-    { iSplitL ""; first iFrame "#".
-      iIntros.
-      iExists (True)%I.
-      iSplitL "".
-      { iIntros "!> _".
-        iPureIntro.
-        by eexists. }
-      iSplitL "".
-      { iIntros (???) "[_ [full1 _]] [[_ [full2 _]] | [_ (% & % & % & [_ [full2 _]])]]";
-          by iPoseProof (ghost_map_auth_valid_2 with "full1 full2") as "[%frac _]". }
-      iSplitL "".
-      { iIntros "!> pers".
-        iSplitL ""; first by iModIntro.
-        iIntros. iFrame. }
-      iSplitL "".
-      { iIntros "!> [full _]".
-        iSplit.
-        - iDestruct "full" as "[? _]".
-          done.
-        - iFrame. }
-      iIntros "[%eq full]".
-      destruct eq as (n' & ? & ?).
-      simplify_eq.
-      iPoseProof (full_pred_withdraw with "[%] full receipt") as "[full %]".
-      { by exists n'. }
-      iFrame "%".
+    wp_apply (wp_faa
+                (λ σ_l n_l σ_t, ⌜(0 ≤ n_l)%Z⌝)%I
+                (λ σ_l (n_l: Z), ⌜ eval σ_l #n_l ⌝ ∗ ⎡ full γ σ_l ⎤: dProp Σ)%I
+                [] [] with "[$mapsto receipt]"); last first.
+    { iIntros (? σ_t n_l) "[>%Hf _]".
+      wp_pures.
       iModIntro.
-      iFrame.
-      rewrite Z.add_opp_r.
-      iSplit.
-      { iPureIntro.
-        rewrite -Nat2Z.inj_sub; last done.
-        eexists.
-        split; first done.
-        rewrite ?foldl_snoc.
-        lia. }
-      iSplit; first by iModIntro.
-      iPureIntro.
-      by eexists.
-    }
-    iIntros "!>" (??) "[post #mapsto]".
-    iPoseProof (post_fence_flush_free with "post") as "(% & % & %)".
-    wp_pures.
-    iModIntro.
-    iApply "HΦ".
-    simplify_eq.
+      by iApply "HΦ". }
+    iIntros (σ_l n_l) "_".
+    iSplitR "receipt".
+    { iIntros (??) "!> (% & % & %)". by iExists _. }
+    iExists (σ_l ++ [inr n]).
+    iSplitR.
+    { iIntros "!> _". iPureIntro. by apply prefix_app_r. }
+    iSplitR.
+    { iIntros (σ_n v_n) "_ [_ full1] disj".
+      iDestruct "full1" as "[auth1 _]".
+      iDestruct "disj" as "[[_ [auth2 _]] | [_ (% & % & % & [_ [auth2 _]])]]";
+        iDestruct (ghost_map_auth_valid_2 with "auth1 auth2") as %[Hv _]; done. }
+    iSplitR.
+    { iIntros "!> [%Heval full]". by iFrame. }
+    iIntros "#seen [(%n_l' & % & %) full] !>".
+    simplify_map_eq.
+    iDestruct (withdraw_impl n n_l' σ_l with "full receipt") as "[fullσt %Hnv]".
+    { exists n_l'. done. }
+    iFrame "∗#".
     iPureIntro.
-    lia.
+    split; last lia.
+    exists (n_l' - n).
+    split.
+    - f_equal. by rewrite Nat2Z.inj_sub.
+    - unfold wsum, dsum in *. rewrite !foldl_snoc /=. lia.
   Qed.
-
-  Lemma receipt_nextgen n:
-    receipt n ⊢ nextgen $ receipt n.
-  Proof. Abort.
-
-  Lemma is_bank_nextgen:
-    is_bank ⊢ nextgen is_bank.
-  Proof. Abort.
-
-  Lemma receipt_split n1 n2:
-    receipt n1 ∗ receipt n2 ⊣⊢ receipt (n1 + n2).
-  Proof. Abort.
-
-End Bank.
+End bank_spec.
