src/examples/optimised_durable_mp.v
@@ -1,25 +1,24 @@
-(* This is a variant of [durable_mp.v] where the flush and fence in the left
-thread is moved to the right thread. *)
+(* This is a variant of [durable_mp.v] where the flush and fence in the writing
+   thread is moved to the reading thread.
 
-From iris.proofmode Require Import ltac_tactics.
+   The writing thread ([leftProg] below) writes [x] and then publishes [y]
+   *without* flushing/fencing [x]. The reading thread ([rightProg] below), upon
+   observing [y = true], performs the flush and fence itself before recording an
+   acknowledgement in [z].
+
+   Because the flush/fence now happens in the reader, the message-passing
+   protocol for [y] can only transfer a [store_lb] for [x] (not a persisted
+   [flush_lb]); the [flush_lb] is established by the reader and handed on to [z].
+
+ * This file is ported with help from claude code. *)
+From iris_named_props Require Import named_props.
 From iris.algebra Require Import excl.
-From PerennialNG.program_logic Require Import staged_invariant.
 
-From self.base Require Import primitive_laws.
-From self.lang Require Import lang.
-From self.high Require Import dprop.
-
-From self.lang Require Import notation lang.
-From self.algebra Require Import view.
-From self.base Require Import primitive_laws class_instances crash_borrow.
-From self.high Require Import proofmode wpc_proofmode.
-From self.high Require Import crash_weakestpre modalities weakestpre
-     weakestpre_na weakestpre_at recovery_weakestpre protocol crash_borrow no_buffer
-     abstract_state_instances locations protocol or_lost.
-From self.high.modalities Require Import fence no_buffer.
+From self.high.lib Require Import abstract_state abstract_state_instances.
+From self.high Require Import protocol wpc_proofmode.
+From self.high Require Import recovery_weakestpre adequacy.
 
 Section program.
-
   Definition leftProg (x y : loc) : expr :=
     #x <-_NA #true ;;
     (* No flush or fence here. *)
@@ -34,303 +33,694 @@ Section program.
     else #().
 
   Definition prog (x y z : loc) : expr :=
-    Fork (rightProg x y z) ;; leftProg x y.
+    Fork (leftProg x y) ;; rightProg x y z.
 
-  Definition recovery x z : expr :=
-    if: !_NA z = #true
-    then assert: !_NA x = #true
+  Definition recovery (x z : loc) : expr :=
+    if: !_NA #z = #true
+    then assert: !_NA #x = #true
     else #().
-
 End program.
 
+Class tokenG (Σ: gFunctors) (Ω: gGenCmras Σ) := {
+  token_inG :: genInDepsG Σ Ω (exclR unitO) [#];
+}.
+
+Definition token_trans: exclR unitO → exclR unitO := id.
+
 Section proof.
-  Context `{nvmG Σ, inG Σ (exclR unitO)}.
-  Context `{!stagedG Σ}.
+  Context `{!nvmBaseGS Σ Ω, !nvmHighGS Σ Ω, !PerennialG Σ, !tokenG Σ Ω}.
+  Context (x y z : loc) (γ__x γ__y γ__z : gname).
 
-  Context (x y z : loc) (γ__ex : gname).
-
-  Definition prot_x : LocationProtocol bool :=
-    {| p_inv (b : bool) v := ⌜ v = #b ⌝%I;
+  Definition inv_x : LocationProtocol bool :=
+    {| p_full (b : bool) v := ⌜ v = #b ⌝%I;
+       p_read (b : bool) v := ⌜ v = #b ⌝%I;
+       p_pers (b : bool) v := ⌜ v = #b ⌝%I;
        p_bumper b := b; |}.
 
-  Global Instance prot_x_cond : ProtocolConditions prot_x.
+  #[global] Instance inv_x_cond ℓ : ProtocolConditions ℓ inv_x.
   Proof.
-    split; [apply _|apply _| ].
-    iIntros. by iApply post_crash_flush_pure.
+    split; try apply _; rewrite /p_full /p_read /p_pers /=.
+    - intros.
+      iSplit; first naive_solver.
+      iIntros "[$ _]".
+    - iIntros.
+      iSplit.
+      + by iIntros "!>!> _".
+      + iIntros (??) "!> % % %".
+        by iIntros "!>!> _".
+    - iIntros.
+      by iModIntro.
   Qed.
 
-  Definition pred_y (s : option bool) (v : val) :=
-    match s with
-      None => True
-    | Some b =>
-        match b with
-          false => ⌜ v = #false ⌝ ∗ ⎡ own γ__ex (Excl ()) ⎤
-        | true => ⌜ v = #true ⌝ ∗ store_lb x prot_x true
-        end
-    end%I.
+  Definition token_pack γ: dProp Σ := ⎡ gen_own γ (Excl ()) ∗ rely_self γ (λ t, t = token_trans) ⎤.
 
-  Definition prot_y := {| p_inv := pred_y; p_bumper _ := None; |}.
-
-  Global Instance prot_y_cond : ProtocolConditions prot_y.
+  Lemma token_pack_alloc:
+    ⊢ |==> ∃ γ, token_pack γ.
   Proof.
-    split; first apply _.
-    - intros [|]; apply _.
-    - iIntros (??) "H /=". iApply post_crash_flush_nodep. done.
+    iMod (own_gen_alloc (DS := [#]) (Excl ()) [#] [##] with "[]") as (γ) "[Hown Htok]".
+    { done. }
+    { iIntros (Hcontr). inversion Hcontr. }
+    iMod (token_strengthen_promise_0_deps _ _ (λ t, t = token_trans) with "Htok") as "Htok"; auto.
+    { intros; done. }
+    { exists id. split; last done.
+      apply _. }
+    iModIntro.
+    iExists γ.
+    iFrame.
+    iApply (rely_to_rely_self).
+    by iApply token_to_rely.
   Qed.
 
-  Definition prot_z :=
-    {| p_inv (b : bool) (v : val) :=
-        match b with
-          false => ⌜ v = #false ⌝ ∗ ⎡ own γ__ex (Excl ()) ⎤
-        | true => ⌜ v = #true ⌝ ∗ flush_lb x prot_x true
+  Lemma token_pack_excl γ:
+    token_pack γ -∗ token_pack γ -∗ False.
+  Proof.
+    iIntros "[own1 _] [own2 _]".
+    iDestruct (gen_own_valid_2 with "[$] [$]") as %[]%exclusive_l.
+  Qed.
+
+  #[global] Instance token_nextgen γ:
+    nextgen.IntoNextgen (token_pack γ) (token_pack γ).
+  Proof.
+    rewrite /nextgen.IntoNextgen.
+    iIntros "[own rely]".
+    iModIntro.
+    iDestruct "own" as (t) "[picked own]".
+    iDestruct "rely" as "[$ (% & % & picked')]".
+    iPickedInAgree "picked picked'".
+    subst.
+    rewrite /token_trans /=.
+    done.
+  Qed.
+
+  #[global] Instance token_nextgen_flush γ:
+    IntoNGFlush (token_pack γ) (token_pack γ).
+  Proof.
+    rewrite /IntoNGFlush.
+    iIntros "[own rely]".
+    iApply nextgen_flush_nextgen.
+    iModIntro.
+    iDestruct "own" as (t) "[picked own]".
+    iDestruct "rely" as "[$ (% & % & picked')]".
+    iPickedInAgree "picked picked'".
+    subst.
+    rewrite /token_trans /=.
+    done.
+  Qed.
+
+  #[global] Instance token_pack_objective γ:
+    Objective (token_pack γ).
+  Proof. apply _. Qed.
+
+  #[global] Instance token_pack_buffer_free γ:
+    BufferFree (token_pack γ).
+  Proof. apply _. Qed.
+
+  (* The bare points-to for [x] at value [true]. Unlike [durable_mp.v]'s
+     [x_pack], this does *not* carry a [flush_lb]: the writing thread does not
+     flush. *)
+  Definition xm : dProp Σ :=
+    ∃ σs, x ↦_{inv_x} (σs ++ [true]).
+
+  #[global] Instance xm_buffer_free:
+    BufferFree (xm).
+  Proof.
+    rewrite /IntoNoBuffer /xm.
+    iIntros "[% xPts]".
+    iModIntro.
+    by iExists _.
+  Qed.
+
+  (* [x_pack] as in [durable_mp.v]: points-to together with a [flush_lb]. This is
+     established by the *reader* (after it flushes and fences) and stored into
+     [z]. *)
+  Definition x_pack: dProp Σ :=
+    xm ∗ flush_lb x inv_x true.
+
+  #[global] Instance x_pack_buffer_free:
+    BufferFree (x_pack).
+  Proof.
+    rewrite /IntoNoBuffer /x_pack /xm.
+    iIntros "[[% xPts] #xFlush]".
+    iModIntro.
+    iSplit; last done.
+    by iExists _.
+  Qed.
+
+  #[global] Instance x_pack_nextgen_flush:
+    IntoNGFlush (x_pack) (x_pack).
+  Proof.
+    rewrite /IntoNGFlush /x_pack /xm.
+    iIntros "[[% xPts] #xFlush]".
+    iModIntro.
+    iDestruct "xFlush" as "[xPers (% & % & xCrashed)]".
+    assert (σ__pc = true) as -> by done.
+    iDestruct (crashed_in_if_rec inv_x with "[$] [$]") as (???) "[xCrashed' xPts]".
+    iDestruct (crashed_in_agree with "[$] [$]") as "->".
+    rewrite /p_bumper list_fmap_id /=.
+    iSplit; last by iApply persist_lb_to_flush_lb.
+    iExists _. iApply "xPts".
+  Qed.
+
+  Opaque xm x_pack token_pack.
+
+  (* [y] is an [option bool] location so that it can [bumper] to [None] after a
+     crash: it transfers only a [store_lb] (flush-free) and a bare points-to
+     [xm] (behind a token), neither of which survives a crash on their own. *)
+  Definition inv_y : LocationProtocol (option bool) :=
+    {| p_full (s : option bool) (v : val) :=
+        match s with
+        | None => True
+        | Some false => ⌜ v = #false ⌝ ∗ token_pack γ__y
+        | Some true => ⌜ v = #true ⌝ ∗ store_lb x inv_x true ∗ (xm ∨ token_pack γ__x)
         end%I;
-      p_bumper := id; |}.
+       p_read (s : option bool) (v : val) :=
+        match s with
+        | None => True
+        | Some false => ⌜ v = #false ⌝ ∗ token_pack γ__y
+        | Some true => ⌜ v = #true ⌝ ∗ store_lb x inv_x true ∗ (xm ∨ token_pack γ__x)
+        end%I;
+       p_pers (s : option bool) (v : val) := True%I;
+       p_bumper _ := None; |}.
 
-  Global Instance prot_z_cond : ProtocolConditions prot_z.
+  #[global] Instance inv_y_cond ℓ : ProtocolConditions ℓ inv_y.
   Proof.
-    split; first apply _.
-    - intros [|]; apply _.
-    - iIntros ([|] ?); simpl.
-      * iIntros "[% lb]". iModIntro.
-        iDestruct "lb" as "(le & ?)".
-        iFrame "%".
-        iApply persist_lb_to_flush_lb. iFrame.
-      * iIntros "[% H]". iModIntro. iFrame. done.
+    split.
+    - intros ?? _. done.
+    - intros [[|]|] v; apply _.
+    - intros [[|]|] v; apply _.
+    - intros [[|]|] v; apply _.
+    - intros s v. rewrite /p_full /p_read /=.
+      iSplit.
+      + iIntros "$". iIntros "$".
+      + iIntros "[$ _]".
+    - iIntros "_" (σ_p v_p σ_f v_f) "%le Hpers Hfull".
+      iSplit.
+      + iModIntro. iModIntro. iIntros "_". by iSplit.
+      + iIntros (σ_c v_c) "!> _ % %". iModIntro. iModIntro. iIntros "_". by iSplit.
+    - iIntros (s v) "_". by iModIntro.
+  Qed.
+
+  Definition inv_z :=
+    {| p_full (b : bool) (v : val) :=
+        ⌜ v = #b ⌝ ∗
+        if b
+        then flush_lb x inv_x true ∗ (x_pack ∨ token_pack γ__z)
+        else True;
+       p_read (b: bool) (v: val) :=
+        ⌜ v = #b ⌝ ∗
+        if b
+        then flush_lb x inv_x true ∗ (x_pack ∨ token_pack γ__z)
+        else True;
+       p_pers (b: bool) (v: val) := ⌜ v = #b ⌝%I;
+       p_bumper := id; |}%I.
+
+  #[global] Instance inv_z_cond ℓ : ProtocolConditions ℓ inv_z.
+  Proof.
+    split; try apply _; rewrite /p_full /p_read /p_pers /=.
+    - intros.
+      iSplit.
+      + iIntros "$".
+        iIntros "$".
+      + iIntros "[$ _]".
+    - iIntros "_" (??????) "[% H]".
+      simplify_map_eq.
+      iSplit.
+      + destruct (σ_f); iIntros "!>!> _"; last naive_solver.
+        iSplitL; last done.
+        iSplitR; first done.
+        iDestruct "H" as "[[xPer _] $]".
+        by iApply persist_lb_to_flush_lb.
+      + iIntros (??) "!> [% H] % %".
+        simplify_map_eq.
+        destruct (σ_c); iIntros "!>!> _"; last naive_solver.
+        iSplitL; last done.
+        iSplitR; first done.
+        iDestruct "H" as "[[xPer _] $]".
+        by iApply persist_lb_to_flush_lb.
+    - iIntros ([|] ?) "[% H] !>"; last done.
+      subst v.
+      iSplitR; first done.
+      iDestruct "H" as "[[xPer _] $]".
+      by iApply persist_lb_to_flush_lb.
   Qed.
 
   (* Note: The recovery code does not use the [y] location, hence the crash
   condition does not mention [y] as we don't need it to be available after a
   crash. *)
   Definition crash_condition : dProp Σ :=
-    ∃ (xss zss : list bool) (bx bz : bool),
-      "%xLast" ∷ ⌜ last xss = Some bx ⌝ ∗
-      "%zLast" ∷ ⌜ last zss = Some bz ⌝ ∗
-      "#xPer" ∷ persist_lb x prot_x bx ∗
-      "#zPer" ∷ persist_lb z prot_z bz ∗
-      x ↦_{prot_x} xss ∗
-      z ↦_{prot_z} zss.
+    ∃ (σ__x σ__z: bool) (σs__z: list bool),
+      "xPer" ∷ persist_lb x inv_x σ__x ∗
+      "x_or_token" ∷ ((∃ σs__x, x ↦_{ inv_x } (σs__x ++ [σ__x])) ∨ token_pack γ__z) ∗
+      "#zPer" ∷ persist_lb z inv_z σ__z ∗
+      "zPts" ∷ z ↦_{inv_z} (σs__z ++ [σ__z]).
 
-  Definition left_crash_condition : dProp Σ :=
-    ∃ xss (bx : bool),
-      "%xLast" ∷ ⌜ last xss = Some bx ⌝ ∗
-      "#xPer" ∷ persist_lb x prot_x bx ∗
-      "xPts" ∷ x ↦_{prot_x} xss.
-
-  Definition right_crash_condition : dProp Σ :=
-    ∃ zss (bz : bool),
-      "%zLast" ∷ ⌜ last zss = Some bz ⌝ ∗
-      "#zPer" ∷ persist_lb z prot_z bz ∗
-      "zPts" ∷ z ↦_{prot_z} zss.
-
-  Lemma left_crash_condition_impl (sx : list bool) :
-    persist_lb x prot_x false -∗
-    x ↦_{prot_x} sx -∗
-    <PC> left_crash_condition.
+  Lemma crash_condition_impl σ__x σ__z σs__z:
+    persist_lb x inv_x σ__x -∗
+    token_pack γ__z -∗
+    persist_lb z inv_z σ__z -∗
+    z ↦_{inv_z} (σs__z) -∗
+    <NG> crash_condition.
   Proof.
-    iIntros "xPer xPts".
+    iIntros "#xPer tok #zPer zPts".
     iModIntro.
-    iDestruct "xPer" as "[#xPer (% & % & #xRec)]".
-    iDestruct (crashed_in_if_rec with "xRec xPts") as (???) "[cras xPts]".
-    iDestruct (crashed_in_agree with "xRec cras") as %->.
-    iDestruct (crashed_in_persist_lb with "xRec") as "#per2".
-    iExists _, _.
-    iFrame "xPts per2".
-    iPureIntro.
-    rewrite last_snoc.
-    done.
+    iDestruct "zPer" as "[zPer' (% & % & zCrashed)]".
+    iDestruct (crashed_in_if_rec inv_z with "[$] [$]") as (???) "[zCrashed' zPts]".
+    iDestruct (crashed_in_agree with "[$] [$]") as "->".
+    iDestruct (crashed_in_persist_lb with "zCrashed") as "#zPer".
+    iDestruct "xPer" as "[xPer (% & % & xCrashed)]".
+    rewrite /p_bumper ?list_fmap_id /=.
+    iExists _, σ_c, σs'.
+    iFrame "xPer".
+    iSplitL "tok".
+    - by iRight.
+    - iFrameNamed.
   Qed.
 
-  Lemma right_crash_condition_impl (sz : list bool) :
-    persist_lb z prot_z false -∗
-    z ↦_{prot_z} sz -∗
-    <PC> right_crash_condition.
-  Proof.
-    iIntros "zPer zPts".
-    iModIntro.
-    iDestruct "zPer" as "[#zPer (% & % & #zRec)]".
-    iDestruct (crashed_in_if_rec with "zRec zPts") as (???) "[cras zPts]".
-    iDestruct (crashed_in_agree with "zRec cras") as %->.
-    iDestruct (crashed_in_persist_lb with "zRec") as "#per2".
-    iExists _, _.
-    iFrame "per2 zPts".
-    rewrite last_snoc.
-    done.
-  Qed.
-
-  (* Prove right crash condition. *)
-  Ltac whack_right_cc :=
+  Ltac solve_left_cc :=
     iSplit;
-    first iApply (right_crash_condition_impl with "zPer zPts").
+    first
+      iApply (crash_condition_impl with "xPer tok zPer zPts").
 
-  Ltac whack_left_cc :=
-    iSplit;
-    first iApply (left_crash_condition_impl with "xPer xPts").
-
-  Lemma no_flush_or (P : dProp Σ) Q : <noflush> (P ∨ Q) ⊣⊢ <noflush> P ∨ <noflush> Q.
-  Proof. iModel. rewrite !no_flush_at. rewrite monPred_at_or. naive_solver. Qed.
-
-  Global Instance into_no_flush_or (P P' Q Q' : dProp Σ) :
-    IntoNoFlush P P' → IntoNoFlush Q Q' → IntoNoFlush (P ∨ Q)%I (P' ∨ Q')%I.
-  Proof. rewrite /IntoNoFlush no_flush_or. by intros <- <-. Qed.
-
-  Lemma right_prog_spec s E1 :
-    y ↦_AT^{prot_y} [Some false] -∗
-    persist_lb z prot_z false -∗
-    z ↦_{prot_z} [false] -∗
-    WPC rightProg x y z @ s; E1
-    {{ v, z ↦_{prot_z} [false; true] ∨ z ↦_{prot_z} [false] }}
-    {{ <PC> right_crash_condition }}.
+  Lemma left_prog_spec s E1 :
+    x ↦_{inv_x} [false] -∗
+    y ↦_AT^{inv_y} [Some false] -∗
+    (WPC leftProg x y @ s; E1
+    {{ _, True }}
+    {{ True }}).
   Proof.
-    iIntros "#yPts #zPer zPts".
-    (* Evaluate the first load. *)
-    rewrite /rightProg.
-    wpc_bind (!_AT _)%E.
-    iApply wpc_atomic_no_mask. whack_right_cc.
-    iApply (wp_load_at_simple _ _ (λ s v, (⌜v = #true⌝ ∗ store_lb x prot_x true) ∨ ⌜v = #false⌝)%I prot_y
-      with "[$yPts]").
-    { iModIntro. iIntros (s' ? incl) "a". simpl.
-      destruct s' as [[|]|]; last done.
-      - iDestruct "a" as "[% #?]". iFrame "#". naive_solver.
-      - iDestruct "a" as "[% O]". naive_solver. }
-    iNext.
-    iIntros (? v) "[yLb' disj]".
-    iDestruct (post_fence_extract' _ (⌜v = #true ∨ v = #false⌝)%I with "disj []") as %[-> | ->].
-    { iIntros "[[-> _]|->]"; naive_solver. }
-    2: {
-      (* We loaded [false] and this case is trivial. *)
-      whack_right_cc.
-      iModIntro.
-      wpc_pures.
-      { iApply (right_crash_condition_impl with "zPer zPts"). }
-      iModIntro.
-      iRight. iFrame. }
-    (* We loaded [true]. *)
-    whack_right_cc.
+    iIntros "xPts #yPts".
+    rewrite /leftProg.
+    wpc_bind (_ <-_NA _)%E.
+    iApply wpc_atomic_no_mask. iSplit; first done.
+    iApply (wp_store_na x _ _ _ _ true with "[$xPts]").
+    { reflexivity. } { done. }
+    { rewrite /inv_x. done. }
+    iNext. iIntros "xPts".
+    iSplit; first done.
     iModIntro.
-    wpc_pures.
-    { iApply (right_crash_condition_impl with "zPer zPts"). }
+    wpc_pures; first done.
 
-    (* Flush *)
-    wpc_bind (Flush _)%E.
-    iApply wpc_atomic_no_mask.
-    whack_right_cc.
+    iDestruct (mapsto_na_store_lb with "xPts") as "#xStore".
 
-    iDestruct (post_fence_flush_free with "disj") as "[[_ storeLb] | %eq]";
-      last inversion eq.
-
-    iApply (wp_flush_lb with "storeLb").
-    iNext.
-    iIntros "(#xLb & _)".
-    whack_right_cc.
-    iModIntro.
-    wpc_pures;
-      first iApply (right_crash_condition_impl with "zPer zPts").
-
-    wpc_bind (Fence).
-    iApply wpc_atomic_no_mask. whack_right_cc.
-    iApply wp_fence. do 2 iModIntro.
-    (* iDestruct "disj" as "[[_ #xLb] | %]"; last congruence. *)
-    whack_right_cc.
-    iModIntro.
-    wpc_pures.
-    { iApply (right_crash_condition_impl with "zPer zPts"). }
-
-    iApply wpc_atomic_no_mask. whack_right_cc.
-    iApply (wp_store_na _ _ _ _ _ true with "[$zPts]"); eauto.
-    { simpl. iFrame "xLb". done. }
-
-    iIntros "!> zPts /=".
-    whack_right_cc.
-    iModIntro.
-    iLeft. iFrame.
+    wpc_bind (_ <-_AT _)%E.
+    iApply wpc_atomic_no_mask. iSplit; first done.
+    iApply (wp_store_at _ inv_y [] (Some false) (Some true) with "[$yPts xPts]").
+    { rewrite /p_full /=.
+      iSplitL.
+      { iSplitPure; first done.
+        iFrame "xStore".
+        iLeft.
+        Transparent xm.
+        iExists [false]. iApply "xPts".
+        Opaque xm. }
+      iSplitPure; first done.
+      iIntros (v_i s_c v_c) "%le". simpl.
+      destruct s_c as [[|]|]; [ | | done ].
+      - iIntros "_". naive_solver.
+      - iIntros "([_ O1] & _ & [_ O2])".
+        iDestruct (token_pack_excl with "O1 O2") as %[]. }
+    iIntros "!> yLb2".
+    iSplit; done.
   Qed.
 
-  Lemma prog_spec :
-    pre_borrow_d ∗
-    (* know_protocol x prot_x ∗ know_protocol y prot_y ∗ know_protocol z prot_z ∗ *)
-    persist_lb x prot_x false ∗
-    x ↦_{prot_x} [false] ∗
-    y ↦_AT^{prot_y} [Some false] ∗
-    persist_lb z prot_z false ∗
-    z ↦_{prot_z} [false] -∗
-    WPC prog x y z @ ⊤
-    {{ v, True }}
-    {{ <PC> crash_condition }}.
+  Lemma prog_spec s:
+    token_pack γ__z ∗
+    token_pack γ__x ∗
+    x ↦_{inv_x} [false] ∗
+    y ↦_AT^{inv_y} [Some false] ∗
+    persist_lb x inv_x false ∗
+    persist_lb z inv_z false ∗
+    z ↦_{inv_z} [false] -∗
+    WPC prog x y z @ s; ⊤
+    {{ v, z ↦_{inv_z} [false; true] ∨ z ↦_{inv_z} [false] }}
+    {{ <NG> crash_condition }}.
   Proof.
-    iIntros "(pb & #xPer & xPts & #yPts & #zPer & zPts)".
+    iIntros "(tok & tok__x & xPts & #yPts & #xPer & #zPer & zPts)".
     rewrite /prog.
 
-    (* We create a crash borrow in order to transfer resources to the forked
-    thread. *)
-    iApply (wpc_crash_borrow_inits _ _ _ _ _ (<PC> right_crash_condition)%I
-             with "pb [zPts]").
-    { iAccu. }
-    { iModIntro. iIntros "zPts".
-      iApply (right_crash_condition_impl with "zPer zPts"). }
-    iIntros "cb".
-
-    iApply (wpc_crash_mono _ _ _ _ _ (<PC> left_crash_condition)%I).
-    { iIntros "L R".
-      iModIntro.
-      iNamed "L".
-      iNamed "R".
-      iExists _, _, _, _.
-      iFrameF (xLast).
-      iFrameF (zLast).
-      iFrame "xPts zPts".
-      iFrame "∗#%". }
-    Unshelve. 2: { apply _. }
-
     wpc_bind (Fork _)%E.
-    iApply (wpc_fork with "[cb]").
-    - (* Show safety of the forked off thread. *)
-      iApply (wpc_crash_borrow_open_modify with "cb"); first done.
-      iNext. iSplit; first done.
-      iIntros "zPts".
-
-      iDestruct (right_prog_spec with "yPts zPer zPts") as "wp".
-      iApply (wpc_mono' with "[] [] wp"); last naive_solver.
-      iIntros (?) "[zPts | zPts]".
-      * iExists (z ↦_{_} (_ : list bool)). iFrame.
-        iSplit; last naive_solver.
-        iIntros "!> zPts".
-        iApply (right_crash_condition_impl with "zPer zPts").
-      * iExists (z ↦_{_} (_ : list bool)). iFrame.
-        iSplit; last naive_solver.
-        iIntros "!> zPts".
-        iApply (right_crash_condition_impl with "zPer zPts").
-    - whack_left_cc. iNext.
-      wpc_pures.
-      { iApply (left_crash_condition_impl with "xPer xPts"). }
-      rewrite /leftProg.
-      wpc_bind (_ <-_NA _)%E.
-      iApply wpc_atomic_no_mask. whack_left_cc.
-      iApply (wp_store_na x _ _ _ _ true with "[$xPts]").
-      { reflexivity. } { done. }
-      { rewrite /prot_x. done. }
-      iNext. iIntros "xPts".
-      whack_left_cc.
+    iApply (wpc_fork with "[xPts]").
+    - (* Show safety of the forked off (writing) thread. *)
+      iDestruct (left_prog_spec with "xPts yPts") as "$".
+    - solve_left_cc. iNext.
+      wpc_pures; first iApply (crash_condition_impl with "xPer tok zPer zPts").
+      rewrite /rightProg.
+      wpc_bind (!_AT _)%E.
+      iApply wpc_atomic_no_mask.
+      solve_left_cc.
+      iApply (wp_load_at_simple _ _
+                (λ (s: option bool) v,
+                   match s with
+                   | Some true => (⌜ v = #true ⌝ ∗ store_lb x inv_x true ∗ xm)%I
+                   | Some false => ⌜ v = #false ⌝%I
+                   | None => False%I
+                   end)
+                inv_y with "[$yPts tok__x]").
+      { iModIntro.
+        iIntros (sL vL) "%le Hr".
+        destruct sL as [[|]|]; simpl in le |- *.
+        - iDestruct "Hr" as "(-> & #store & [xm | tokx])".
+          + iSplitL "xm".
+            * iSplitR; first done. iFrame "store xm".
+            * iSplitR; first done. iFrame "store". iRight. iFrame "tok__x".
+          + iDestruct (token_pack_excl with "tokx tok__x") as %[].
+        - iDestruct "Hr" as "(-> & toky)".
+          iSplitR "toky"; first done.
+          iSplitR; first done. iFrame "toky".
+        - destruct le. }
+      iNext.
+      iIntros (sL vL) "[yPts2 Q]".
+      destruct sL as [[|]|].
+      2: {
+        (* We loaded [false] and this case is trivial. *)
+        iDestruct "Q" as ">->".
+        solve_left_cc.
+        iModIntro.
+        wpc_pures.
+        { iApply (crash_condition_impl with "xPer tok zPer zPts"). }
+        iModIntro.
+        iRight. iFrame "zPts". }
+      2: {
+        (* Impossible: [None] is not reachable. *)
+        iDestruct "Q" as ">[]". }
+      (* We loaded [true]. *)
+      iDestruct "Q" as "(>-> & >#store & xmF)".
+      solve_left_cc.
       iModIntro.
-      wpc_pures;
-        first iApply (left_crash_condition_impl with "xPer xPts").
+      wpc_pures.
+      { iApply (crash_condition_impl with "xPer tok zPer zPts"). }
 
-      iDestruct (mapsto_na_store_lb with "xPts") as "#xStoreLb".
-      wpc_bind (_ <-_AT _)%E.
-      iApply wpc_atomic_no_mask. whack_left_cc.
-      iApply (wp_store_at _ prot_y [] (Some false) (Some true)).
-      { simpl.
-        iFrameF "yPts".
-        iFrame "xStoreLb".
-        iSplitPure. { done. }
-        iSplitPure. { done. }
-        iFrame "#".
-        iIntros (? s_c v_c). simpl.
-        destruct s_c as [[|]|]; [naive_solver| |naive_solver].
-        iIntros "? ([? O1] & [??] & [? O2])".
-        by iDestruct (own_valid_2 with "O1 O2") as %HI%exclusive_l. }
-      iIntros "!> yLb2".
-      whack_left_cc.
-      done.
+      (* Flush *)
+      wpc_bind (Flush _)%E.
+      iApply wpc_atomic_no_mask. solve_left_cc.
+      iApply (wp_flush_lb with "store").
+      iNext.
+      iIntros "(#xFlushF & _)".
+      solve_left_cc.
+      iModIntro.
+      wpc_pures; first iApply (crash_condition_impl with "xPer tok zPer zPts").
+
+      (* The fence: discharges both the pending [xm] and the pending [flush_lb]. *)
+      wpc_bind (Fence)%E.
+      iApply wpc_atomic_no_mask. solve_left_cc.
+      iApply wp_fence. do 2 iModIntro.
+      solve_left_cc.
+      iModIntro.
+      wpc_pures.
+      { iApply (crash_condition_impl with "xPer tok zPer zPts"). }
+
+      iApply wpc_atomic_no_mask. solve_left_cc.
+      iApply (wp_store_na _ inv_z _ _ _ true with "[$zPts xmF xFlushF]"); eauto.
+      { iSplitR; first done.
+        iFrame "xFlushF".
+        iLeft.
+        Transparent x_pack.
+        iFrame "xmF xFlushF".
+        Opaque x_pack. }
+
+      iIntros "!> zPts /=".
+      solve_left_cc.
+      iModIntro.
+      iLeft. iFrame "zPts".
   Qed.
 
+  Instance if_else_persistent {PROP : bi} (b : bool) (P Q : PROP) :
+    Persistent P →
+    Persistent Q →
+    Persistent (if b then P else Q).
+  Proof. intros ??. destruct b; done. Qed.
+
+  Lemma crash_condition_impl' σ__x σ__z σs__z σs__x:
+    persist_lb x inv_x σ__x -∗
+    x ↦_{inv_x} (σs__x) -∗
+    persist_lb z inv_z σ__z -∗
+    z ↦_{inv_z} (σs__z) -∗
+    <NG> crash_condition.
+  Proof.
+    iIntros "#xPer xPts #zPer zPts".
+    iModIntro.
+    iDestruct "zPer" as "[zPer' (% & % & zCrashed)]".
+    iDestruct (crashed_in_if_rec inv_z with "[$] [$]") as (???) "[zCrashed' zPts]".
+    iDestruct (crashed_in_agree with "[$] [$]") as "->".
+    iDestruct (crashed_in_persist_lb with "zCrashed") as "#zPer".
+    iDestruct "xPer" as "[xPer' (% & % & xCrashed)]".
+    iDestruct (crashed_in_if_rec inv_x with "xCrashed [$]") as (???) "[xCrashed' xPts]".
+    iDestruct (crashed_in_agree with "xCrashed' xCrashed") as "->".
+    iDestruct (crashed_in_persist_lb with "xCrashed") as "#xPer".
+    rewrite /p_bumper ?list_fmap_id /=.
+    iExists _, _, _.
+    iFrame "xPer".
+    iSplitL "xPts"; last iFrameNamed.
+    iLeft.
+    by iExists _.
+  Qed.
+
+  Lemma recovery_prog_spec s E :
+    crash_condition -∗
+    WPC recovery x z @ s; E
+      {{ _, True }} {{ <NG> crash_condition }}.
+  Proof.
+    iNamed 1.
+    iDestruct "x_or_token" as "[[% xPts] | tok]".
+    - rewrite /recovery.
+      wpc_bind (!_NA _)%E.
+      iApply wpc_atomic_no_mask.
+      iSplit.
+      { iApply (crash_condition_impl' with "xPer xPts zPer zPts"). }
+      iApply (wp_load_na _ _ _ _ (λ v, (⌜ v = #true ⌝ ∗ flush_lb x inv_x true) ∨ ⌜ v = #false ⌝)%I with "[$zPts]").
+      { apply last_snoc. }
+      { iModIntro.
+        simpl.
+        iIntros (?) "[-> H]".
+        destruct σ__z; last naive_solver.
+        iDestruct "H" as "[#xFlush H]".
+        iSplitR; last naive_solver.
+        naive_solver. }
+      iNext. iIntros (?) "[zPts H]".
+      iDestruct "H" as "[[-> #xFlush] | ->]".
+      + iPoseProof (mapsto_na_flush_lb_incl with "xFlush xPts") as "%Horder".
+        assert (σ__x = true) as -> by done.
+        iSplit.
+        { iModIntro. iApply (crash_condition_impl' with "xPer xPts zPer zPts"). }
+        iModIntro.
+        rewrite /assert.
+        wpc_pures.
+        { iApply (crash_condition_impl' with "xPer xPts zPer zPts"). }
+        wpc_bind (!_NA _)%E.
+        iApply wpc_atomic_no_mask. iSplit.
+        { iApply (crash_condition_impl' with "xPer xPts zPer zPts"). }
+        iApply (wp_load_na with "[$xPts]").
+        { apply last_snoc. }
+        { iModIntro. simpl.
+          iIntros (?). iIntros "#H". iFrame "H". rewrite right_id. iApply "H". }
+        iNext. iIntros (?) "[xPts ->]".
+        iSplit.
+        { iApply (crash_condition_impl' with "xPer xPts zPer zPts"). }
+        iModIntro.
+        wpc_pures.
+        { iApply (crash_condition_impl' with "xPer xPts zPer zPts"). }
+        done.
+      + iSplit.
+        { iApply (crash_condition_impl' with "xPer xPts zPer zPts"). }
+        iModIntro.
+        wpc_pures.
+        { iApply (crash_condition_impl' with "xPer xPts zPer zPts"). }
+        done.
+    - rewrite /recovery.
+      wpc_bind (!_NA _)%E.
+      iApply wpc_atomic_no_mask.
+      iSplit.
+      { iApply (crash_condition_impl with "xPer tok zPer zPts"). }
+      iApply (wp_load_na _ _ _ _ (λ v, (⌜ v = #true ⌝ ∗ x_pack) ∨ (⌜ v = #false ⌝ ∗ token_pack γ__z))%I with "[$zPts tok]").
+      { apply last_snoc. }
+      { iModIntro.
+        simpl.
+        iIntros (?) "[-> H]".
+        destruct σ__z; last naive_solver.
+        iDestruct "H" as "[$ [H | H]]"; last iDestruct (token_pack_excl with "[$] [$]") as %[].
+        iSplitL "H".
+        - iLeft. naive_solver.
+        - iSplitPure; first done.
+          by iRight. }
+      iNext. iIntros (?) "[zPts H]".
+      iDestruct "H" as "[[-> H] | [-> tok]]".
+      + Transparent x_pack.
+        iDestruct ("H") as "[xm xFlush]".
+        Transparent xm.
+        iDestruct "xm" as "[% xPts]".
+        Opaque xm x_pack.
+        iSplit.
+        { iModIntro. iApply (crash_condition_impl' with "xPer xPts zPer zPts"). }
+        iModIntro.
+        rewrite /assert.
+        wpc_pures.
+        { iApply (crash_condition_impl' with "xPer xPts zPer zPts"). }
+        wpc_bind (!_NA _)%E.
+        iApply wpc_atomic_no_mask. iSplit.
+        { iApply (crash_condition_impl' with "xPer xPts zPer zPts"). }
+        iApply (wp_load_na with "[$xPts]").
+        { apply last_snoc. }
+        { iModIntro. simpl.
+          iIntros (?). iIntros "#H". iFrame "H". rewrite right_id. iApply "H". }
+        iNext. iIntros (?) "[xPts ->]".
+        iSplit.
+        { iApply (crash_condition_impl' with "xPer xPts zPer zPts"). }
+        iModIntro.
+        wpc_pures.
+        { iApply (crash_condition_impl' with "xPer xPts zPer zPts"). }
+        done.
+      + iSplit.
+        { iApply (crash_condition_impl with "xPer tok zPer zPts"). }
+        iModIntro.
+        wpc_pures.
+        { iApply (crash_condition_impl with "xPer tok zPer zPts"). }
+        done.
+  Qed.
+
+  Definition φ (v: val): Prop := True.
+
+  Lemma simple_prog_spec (s: stuckness):
+    token_pack γ__z ∗
+    token_pack γ__x ∗
+    x ↦_{inv_x} [false] ∗
+    y ↦_AT^{inv_y} [Some false] ∗
+    persist_lb x inv_x false ∗
+    persist_lb z inv_z false ∗
+    z ↦_{inv_z} [false] -∗
+    WPC prog x y z @ s; ⊤
+    {{ v, ⌜ φ v ⌝ }}
+    {{ <NG> crash_condition }}.
+  Proof.
+    iIntros "Hpre".
+    iApply (wpc_mono'); last by iApply prog_spec.
+    - done.
+    - iIntros.
+      done.
+    - by iIntros.
+  Qed.
+
+  Lemma simple_rec_spec (s: stuckness):
+    (<NG> crash_condition) -∗
+    (<NG> (WPC recovery x z @ s; ⊤
+    {{ v, ⌜ φ v ⌝ }}
+    {{ <NG> crash_condition }})).
+  Proof.
+    iApply nextgen.nextgen_mono.
+    iIntros "Hpre".
+    iApply (wpc_mono'); last by iApply recovery_prog_spec.
+    - done.
+    - iIntros.
+      done.
+    - by iIntros.
+  Qed.
+
+  Lemma wpr_spec (s: stuckness):
+    (token_pack γ__z ∗
+     token_pack γ__x ∗
+     x ↦_{inv_x} [false] ∗
+     y ↦_AT^{inv_y} [Some false] ∗
+     persist_lb x inv_x false ∗
+     persist_lb z inv_z false ∗
+     z ↦_{inv_z} [false]) ⊥ -∗
+    validV ∅ -∗
+    wpr s ⊤ (prog x y z `at` ⊥) (recovery x z `at` ⊥)
+      (λ v, ⌜ φ v.(val_val) ⌝)%I
+      True%I
+      (λ v, ⌜ φ v.(val_val) ⌝)%I.
+  Proof.
+    iIntros "Hpre HvalidV".
+    iPoseProof (idempotence_wpr with "[Hpre] [] HvalidV") as "Hwpr".
+    - simpl.
+      iApply (simple_prog_spec s with "Hpre").
+    - iIntros "!>".
+      rewrite monPred_at_wand.
+      iIntros (TV ?) "cc".
+      iModIntro.
+      iApply (simple_rec_spec s with "cc").
+    - simpl.
+      iApply (wpr_strong_mono with "Hwpr").
+      naive_solver.
+  Qed.
 End proof.
+
+Section closed_proof.
+  Context `{!nvmBaseGS Σ Ω, !nvmHighGS Σ Ω, !PerennialG Σ, !tokenG Σ Ω}.
+  Lemma closed_wpr_spec (s: stuckness) x y z:
+    ⊢ |==> ∃ γ__x γ__y γ__z,
+      (x ↦_{inv_x} [false] ∗
+       persist_lb x inv_x false ∗
+       y ↦_AT^{inv_y x γ__x γ__y} [Some false] ∗
+       z ↦_{inv_z x γ__z} [false] ∗
+       persist_lb z (inv_z x γ__z) false) ⊥ -∗
+      validV ∅ -∗
+      ((inv_x.(p_full) false #false ∗ inv_x.(p_pers) false #false) ∗
+       ((inv_y x γ__x γ__y).(p_full) (Some false) #false ∗ (inv_y x γ__x γ__y).(p_pers) (Some false) #false) ∗
+       ((inv_z x γ__z).(p_full) false #false ∗ (inv_z x γ__z).(p_pers) false #false)) ⊥ ∗
+      wpr s ⊤ (prog x y z `at` ⊥) (recovery x z `at` ⊥)
+        (λ v, ⌜ φ v.(val_val) ⌝)%I
+        True%I
+        (λ v, ⌜ φ v.(val_val) ⌝)%I.
+  Proof.
+    iMod (token_pack_alloc $! ⊥) as (γ__x) "x_pack".
+    iMod (token_pack_alloc $! ⊥) as (γ__y) "y_pack".
+    iMod (token_pack_alloc $! ⊥) as (γ__z) "z_pack".
+    iModIntro.
+    iExists γ__x, γ__y, γ__z.
+    monPred_simpl.
+    Opaque persist_lb mapsto_at.
+    iIntros "(xPts & #xPer & #yPts & zPts & #zPer) #validV".
+    iSplitR "x_pack z_pack xPts zPts".
+    - rewrite /p_full /p_pers /=.
+      iSplit; first naive_solver.
+      iSplit; last naive_solver.
+      iSplit; last naive_solver.
+      iSplit; first naive_solver.
+      iFrame "y_pack".
+    - iApply (wpr_spec with "[-]"); last done.
+      monPred_simpl.
+      iFrame "xPts zPts yPts xPer zPer z_pack x_pack".
+  Qed.
+End closed_proof.
+
+Section adequacy.
+  Context (x y z: loc) (s: stuckness).
+  Context (Build_nvmHighGpreS: ∀ Σ Ω (nvmBase: nvmBaseGS Σ Ω), nvmHighGpreS Σ Ω).
+  Definition σ__na: gmap loc val := {[ x := #false; z := #false ]}.
+  Definition σ__at: gmap loc val := {[ y := #false ]}.
+  Definition PV: view.view := {[ x := MaxNat 0; y := MaxNat 0; z := MaxNat 0 ]}.
+
+  Opaque mapsto_at mapsto_na persist_lb token_pack.
+
+  Theorem optimised_durable_mp_safe Σ Ω `{!nvmBaseGpreS Σ Ω, !Perennial_preG Σ Ω} `{!tokenG Σ Ω}:
+    x ≠ y ∧ x ≠ z ∧ y ≠ z →
+    recv_adequate s (prog x y z `at` ⊥) (recovery x z `at` ⊥) (initial_heap (σ__at ∪ σ__na), PV) (λ v _, φ v.(val_val)) (λ v _, φ v.(val_val)).
+  Proof using Build_nvmHighGpreS.
+    intros Hdistinct.
+    apply (high_recv_adequacy_simple Build_nvmHighGpreS Σ Ω).
+    { set_solver. }
+    { set_solver. }
+    intros ???.
+    iMod (closed_wpr_spec s x y z) as (γ__x γ__y γ__z) "Hwpr".
+    iModIntro.
+    iExists {[ y := adequacy_alloc.MkLocInfo Σ Ω Hbase Hhigh _ _ _ _ (inv_y x γ__x γ__y) _ (Some false) ]}.
+    iExists {[ x := adequacy_alloc.MkLocInfo Σ Ω Hbase Hhigh _ _ _ _ inv_x _ false; z := adequacy_alloc.MkLocInfo Σ Ω Hbase Hhigh _ _ _ _ (inv_z x γ__z) _ false ]}.
+    iSplit; first (iPureIntro; set_solver).
+    iSplit; first (iPureIntro; set_solver).
+    iIntros "Hat Hna validV".
+    rewrite /adequacy_alloc.init_at_assertions /adequacy_alloc.init_na_assertions.
+    iEval (rewrite big_sepM2_singleton /=) in "Hat".
+    iDestruct "Hat" as "[#pPer #yPts]".
+    rewrite big_sepM2_insert ?lookup_insert_ne //; [ | naive_solver | naive_solver ].
+    rewrite big_sepM2_singleton /=.
+    iDestruct "Hna" as "[[#xPer xPts] [#zPer zPts]]".
+    iDestruct ("Hwpr" with "[$xPts $xPer $yPts $zPts $zPer] validV") as "[(_ & [[_ y_pack] _] & _) Hwpr]".
+    rewrite /adequacy_alloc.init_prots.
+    rewrite big_sepM2_singleton /=.
+    rewrite big_sepM2_insert ?lookup_insert_ne //; [ | naive_solver | naive_solver ].
+    rewrite big_sepM2_singleton /=.
+    iFrame.
+    naive_solver.
+  Qed.
+End adequacy.
+
+Print Assumptions optimised_durable_mp_safe.
